ems/ModSem.v
@@ -264,13 +264,59 @@ Section LEMMAS.
     extensionalities. ss.
   Qed.
   
+  Lemma translate_emb_unwrapU
+    R run_ (r: option R)
+  :
+    translate (emb_ run_) (unwrapU r) = unwrapU r
+  .
+  Proof.
+    unfold unwrapU. destruct r.
+    - apply translate_emb_ret.
+    - apply translate_emb_triggerUB.
+  Qed.
+
+  Lemma translate_emb_unwrapN
+    R run_ (r: option R)
+  :
+    translate (emb_ run_) (unwrapN r) = unwrapN r
+  .
+  Proof.
+    unfold unwrapN. destruct r.
+    - apply translate_emb_ret.
+    - apply translate_emb_triggerNB.
+  Qed.
+
+  Lemma translate_emb_assume
+    run_ P
+  :
+    translate (emb_ run_) (assume P) = assume P
+  .
+  Proof.
+    unfold assume. rewrite translate_emb_bind.
+    rewrite translate_emb_eventE. f_equal.
+    extensionalities.
+    rewrite translate_emb_ret. et.
+  Qed.
+
+  Lemma translate_emb_guarantee
+    run_ P
+  :
+    translate (emb_ run_) (guarantee P) = guarantee P
+  .
+  Proof.
+    unfold guarantee. rewrite translate_emb_bind.
+    rewrite translate_emb_eventE. f_equal.
+    extensionalities.
+    rewrite translate_emb_ret. et.
+  Qed.
+
   Lemma translate_emb_ext
     T run_ (itr0 itr1: itree _ T)
     (EQ: itr0 = itr1)
   :
     translate (emb_ run_) itr0 = translate (emb_ run_) itr1
   .
-
+  Proof. subst. refl. Qed.
   
 
 End LEMMAS.
@@ -744,22 +790,23 @@ Section AUX.
       (mk_box interp_Es_ext)
   .
 
-  Global Program Instance transl_emb_rdb: red_database (mk_box (@translate)) :=
+  Global Program Instance translate_emb_rdb: red_database (mk_box (@translate)) :=
     mk_rdb
       0
-      (mk_box ModSem.transl_emb_bind)
-      (mk_box ModSem.transl_emb_tau)
-      (mk_box ModSem.transl_emb_ret)
-      (mk_box ModSem.transl_emb_sE)
-      (mk_box ModSem.transl_emb_callE)
-      (mk_box ModSem.transl_emb_eventE)
-      (mk_box ModSem.transl_emb_triggerUB)
-      (mk_box ModSem.transl_emb_triggerNB)
-      (mk_box transl_emb_unwrapU)
-      (mk_box transl_emb_unwrapN)
-      (mk_box transl_emb_assume)
-      (mk_box transl_emb_guarantee)
-      (mk_box transl_emb_ext)
+      (mk_box ModSem.translate_emb_bind)
+      (mk_box ModSem.translate_emb_tau)
+      (mk_box ModSem.translate_emb_ret)
+      (mk_box ModSem.translate_emb_sE)
+      (mk_box ModSem.translate_emb_sE)
+      (mk_box ModSem.translate_emb_callE)
+      (mk_box ModSem.translate_emb_eventE)
+      (mk_box ModSem.translate_emb_triggerUB)
+      (mk_box ModSem.translate_emb_triggerNB)
+      (mk_box ModSem.translate_emb_unwrapU)
+      (mk_box ModSem.translate_emb_unwrapN)
+      (mk_box ModSem.translate_emb_assume)
+      (mk_box ModSem.translate_emb_guarantee)
+      (mk_box ModSem.translate_emb_ext)
   .
 
 
